% JUMP TO LINE 60, 75
\documentclass[preview, margin=0.6in]{standalone}
\usepackage[letterpaper,portrait,top=0.4in, left=0.6in, right=0.6in, bottom=1in]{geometry}

\usepackage{amsmath, amsfonts, amsthm, amssymb}
\usepackage{graphicx, float}
\usepackage{mathtools}
\usepackage{titlesec}
\usepackage{interval}
\usepackage{hyperref}
\usepackage{siunitx}
\usepackage{titling}
\usepackage{vwcol}
\usepackage{setspace}
\usepackage{empheq}
\usepackage{cancel}
\usepackage{esdiff}
\usepackage{multicol}
\usepackage{mdframed}
\usepackage{esdiff}
\usepackage{tikzsymbols}
\usepackage{multicol}
\usepackage{tikz}
\usepackage{varwidth}
\usepackage{parskip}
\usepackage{pgfplots}
\pgfplotsset{compat=1.18}
\intervalconfig {
	soft open fences
}

\newcommand{\alignedintertext}[1]{%
  \noalign{%
    \vtop{\hsize=\linewidth#1\par
    \expandafter}%
    \expandafter\prevdepth\the\prevdepth
  }%
}

\newtheorem{lemma}{Lemma}

\renewcommand{\qedsymbol}{\Smiley[1.3]}
\newcommand*{\problem}[1]{\section*{Problem #1}}
\newcommand*{\aps}{\section*{AP Corner}}
\newcommand*{\deriv}[1][x]{\ensuremath{\dfrac{\mathrm{d}}{\mathrm{d}#1}}}
\newcommand*{\floor}[1]{\ensuremath{\lfloor #1\rfloor}}
\newcommand*{\lheqzero}{\ensuremath{\underset{\text{L'H}}{\overset{\left[\frac00\right]}{=}}}}
\newcommand*{\lheqinfty}{\ensuremath{\underset{\text{L'H}}{\overset{\left[\frac{\infty}{\infty}\right]}{=}}}}

\DeclareMathOperator{\DNE}{DNE}
\DeclareMathOperator{\sgn}{sgn}

\DeclareMathOperator{\arccsc}{arccsc}
\DeclareMathOperator{\arcsec}{arcsec}
\DeclareMathOperator{\arccot}{arccot}

%opening

\title{\vspace*{-30pt}Problem Set \# 60}
\author{Jayden Li}
\date{\today}

% \allowdisplaybreaks
\postdisplaypenalty=100000

\begin{document}
\setstretch{1.25}
\fontsize{12pt}{12pt}\selectfont
\setlength{\abovedisplayskip}{0pt}
\setlength{\parindent}{0pt}
\setlength{\parskip}{2ex plus 0.5ex minus 0.2ex}
\maketitle

\problem{2}
\begin{itemize}
	\item[(a)]
		$\begin{aligned}[t]
			\alignedintertext{
			\begin{mdframed}
				$\begin{aligned}[t]
					I(x)&=\exp \int 1\,\mathrm{d}x
					=\exp(x)
				\end{aligned}$
			\end{mdframed}
			}
			\diff yx+y=1
			&\implies \diff yx+1\cdot y=1
			\implies e^x\diff yx+e^xy=e^x
			\implies \deriv e^xy=e^x
			\implies e^xy=e^x+C \\
			&\implies \boxed{y=1+\frac{C}{e^x}}
		\end{aligned}$

	\item[(b)]
		$\begin{aligned}[t]
		    \diff yx=x-y
			&\implies \diff yx+y=x
			\implies e^x\diff yx+e^xy=xe^x
			\implies \int\deriv e^xy \,\mathrm{d}x=\int xe^x\,\mathrm{d}x \\
			&\implies e^xy=xe^x-e^x+C
			\implies \boxed{y=x-1+\frac{C}{e^x}}
		\end{aligned}$

	\item[(e)]
		$\begin{aligned}[t]
			(1+t)\diff ut+u=1+t
			&\implies \diff ut+\frac{1}{1+t}u=1 \\
			\alignedintertext{
			\begin{mdframed}
				$\begin{aligned}[t]
					I(t)&=\exp\int \frac{1}{1+t}\,\mathrm{d}t
					=\exp(\ln|1+t|+C)
					=C(1+t)
				\end{aligned}$
			\end{mdframed}
			}
			&\implies (1+t)\diff ut+u=1+t
			\implies \int\deriv[t] (1+t)u \,\mathrm{d}t=\int\left(1+t\right)\mathrm{d}t \\
			&\implies (1+t)u=t+\frac{t^2}{2}+C
			\implies u=\frac{t}{1+t}+\frac{t^2}{2(1+t)}+\frac{C}{1+t}
		\end{aligned}$
\end{itemize}

\problem{4}
$\begin{aligned}[t]
	\diff yx +P(x)y=Q(x)y^n
	&\implies \left[\begin{aligned}
			u&=y^{1-n} \\
			y&=u^{\frac{1}{1-n}} \\
			\mathrm{d}y&=\frac{1}{1-n}u^{\frac{n}{1-n}}\,\mathrm{d}u
	\end{aligned}\right]
	\frac{1}{1-n}\diff ux u^{\frac{n}{1-n}}+P(x)u^{\frac{1}{1-n}}=Q(x)u^{\frac{n}{1-n}} \\
	&\implies u^{\frac{-n}{1-n}}\left(\diff ux u^{\frac{n}{1-n}}+(1-n)P(x)u^{\frac{1}{1-n}}\right)=(1-n)Q(x)u^{\frac{n}{1-n}}u^{\frac{-n}{1-n}} \\
	&\implies \diff ux+(1-n)P(x)u^{\frac{1-n}{1-n}}=(1-n)Q(x) \\
	&\implies \diff ux+(1-n)P(x)u=(1-n)Q(x) \\
\end{aligned}$

\problem{5}
$\begin{aligned}[t]
    \diff yx +\frac 2xy=\frac{y^3}{x^2}
	&\implies \left[\begin{aligned}
			u&=y^{-2} \\
			y&=u^{-1/2} \\
			\diff yx&=-\frac12 u^{-3/2}\diff ux
	\end{aligned}\right]
	-\frac12 u^{-3/2}\diff ux+\frac2xu^{-1/2}=\frac{\left(u^{-1/2}\right)^3}{x^2} \\
	&\implies u^{3/2}\left(-\frac12 u^{-3/2}\diff ux+\frac2xu^{-1/2}\right)=u^{3/2}\cdot\frac{u^{-3/2}}{x^2}
	\implies -2\left(-\frac12\diff ux+\frac2xu\right)=\frac{1}{x^2}\cdot(-2) \\
	&\implies \diff ux-\frac4xu=-\frac{2}{x^2} \\
	\alignedintertext{
	\begin{mdframed}
		$\begin{aligned}[t]
			I(x)&=\exp \int\left(-\frac4x\right)\mathrm{d}x
			=\left(\exp \ln|x|\right)^{-4}
			=|x|^{-4}
			=x^{-4}
		\end{aligned}$
	\end{mdframed}
	}
	&\implies x^{-4}\diff ux-4x^{-5}u=-2x^{-6}
	\implies \int \deriv[x]\left[x^{-4}u\right]\,\mathrm{d}x=\int\left(-2x^{-6}\right)\mathrm{d}x \\
	&\implies x^4x^{-4}u=\left(\frac{-2}{-5}x^{-5}+C\right)x^4
	\implies \boxed{\frac{1}{y^2}=\frac{2}{5x}+Cx^4}
\end{aligned}$

\end{document}
